instantiation/SealCap.thy
@@ -114,7 +114,7 @@ theorem SemanticsSealCap:
   fixes s auth
   defines "t \<equiv> ucast (getBase (getCapReg auth s)) + ucast (getOffset (getCapReg auth s))"
   assumes prov: "SealCapAction auth cd cd' \<in> actions"
-      and suc: "(KeepDomain actions, s') \<in> NextStates s"
+      and suc: "(PreserveDomain actions, s') \<in> NextStates s"
   shows "Permit_Seal (getPerms (getCapReg auth s))"
         "getTag (getCapReg auth s)"
         "\<not> getSealed (getCapReg auth s)"
